examples/lambda/basics/nomdatatype.sml
@@ -1,0 +1,359 @@
+structure nomdatatype :> nomdatatype =
+struct
+
+  open binderLib HolKernel Parse boolLib generic_termsTheory
+
+(* utility functions *)
+fun rpt_hyp_dest_conj th = let
+  fun foldthis (t, acc) = let
+    fun dc t = let
+      val (c1, c2) = dest_conj t
+    in
+      CONJ (dc c1) (dc c2)
+    end handle HOL_ERR _ => ASSUME t
+  in
+    PROVE_HYP (dc t) acc
+  end
+in
+  HOLset.foldl foldthis th (hypset th)
+end
+
+fun hCONJ th1 th2 =
+    case (hyp th1, hyp th2) of
+      ([h1], [h2]) => let
+        val h12 = ASSUME(mk_conj(h1,h2))
+      in
+        CONJ th1 th2
+             |> PROVE_HYP (CONJUNCT1 h12)
+             |> PROVE_HYP (CONJUNCT2 h12)
+      end
+    | _ => CONJ th1 th2
+
+val FINITE_t = mk_thy_const{Name = "FINITE", Thy = "pred_set",
+                            Ty = (stringSyntax.string_ty --> bool) --> bool}
+
+fun elim_unnecessary_atoms {finite_fv} fths = let
+  fun mainconv t = let
+    val (vs, bod) = strip_forall t
+    val (v,rest) = case vs of
+                     [] => raise mk_HOL_ERR "nomdatatype" "elim_unnecessary_atoms"
+                                            "Not a forall"
+                   | v::vs => (v,vs)
+    val _ = Type.compare(type_of v, stringSyntax.string_ty) = EQUAL orelse
+            raise mk_HOL_ERR "nomdatatype" "elim_unnecessary_atoms"
+                             "Forall not of an atom"
+    val (h, c) = dest_imp bod
+    val _ = free_in v h andalso not (free_in v c) orelse
+            raise mk_HOL_ERR "nomdatatype" "elim_unnecessary_atoms"
+                             "Uneliminable atom"
+    fun PROVE_FINITE t = let
+      open pred_setTheory pred_setSyntax
+      val (v, bod) = dest_exists t
+      val cs = strip_conj bod
+      fun getset t = let
+        val t0 = dest_neg t
+      in
+        if is_in t0 then rand t0 else mk_set [rhs t0]
+      end
+      val sets = map getset cs
+      val union = List.foldl (mk_union o swap) (hd sets) (tl sets)
+      val finite_t = mk_finite union
+      val finite_th =
+        REWRITE_CONV (FINITE_UNION::FINITE_INSERT::FINITE_EMPTY::finite_fv::fths)
+                     finite_t
+      val fresh_exists = MATCH_MP basic_swapTheory.new_exists (EQT_ELIM finite_th)
+                                  |> REWRITE_RULE [IN_UNION, IN_INSERT, NOT_IN_EMPTY,
+                                                   DE_MORGAN_THM, GSYM CONJ_ASSOC]
+    in
+      EQT_INTRO fresh_exists
+    end
+
+    val base = HO_REWR_CONV LEFT_FORALL_IMP_THM THENC
+               LAND_CONV (((CHANGED_CONV EXISTS_AND_REORDER_CONV THENC
+                            RAND_CONV PROVE_FINITE) ORELSEC
+                           PROVE_FINITE)) THENC
+               REWRITE_CONV []
+    fun recurse t = ((SWAP_FORALL_CONV THENC BINDER_CONV recurse) ORELSEC base) t
+  in
+    recurse
+  end t
+in
+  CONV_RULE (ONCE_DEPTH_CONV mainconv)
+end
+
+
+
+val gterm_ty = mk_thy_type {Thy = "generic_terms", Tyop = "gterm",
+                            Args = [beta,alpha]}
+
+local
+  val num_ty = numSyntax.num
+  val numlist_ty = listSyntax.mk_list_type num_ty
+  val string_ty = stringSyntax.string_ty
+in
+val genind_t =
+  mk_thy_const {Thy = "generic_terms", Name = "genind",
+                Ty = (num_ty --> alpha --> bool) -->
+                     (num_ty --> beta --> numlist_ty --> numlist_ty --> bool) -->
+                     num_ty --> gterm_ty --> bool}
+val GVAR_t = mk_thy_const {Thy = "generic_terms", Name = "GVAR",
+                           Ty = string_ty --> alpha --> gterm_ty}
+end
+
+fun first2 l =
+    case l of
+      (x::y::_) => (x,y)
+    | _ => raise Fail "first2: list doesn't have at least two elements"
+
+fun new_type_step1 tyname {vp, lp} = let
+  val list_mk_icomb = uncurry (List.foldl (mk_icomb o swap))
+  val termP = list_mk_icomb (genind_t, [vp,lp,numSyntax.mk_numeral Arbnum.zero])
+  fun termPf x = mk_comb(termP, x)
+  val (gtty,_) = dom_rng (type_of termP)
+  val x = mk_var("x",gtty) and y = mk_var("y", gtty)
+  val (glam_ty, gvar_ty) = first2 (#2 (dest_type gtty))
+  infix /\
+  fun t1 /\ t2 = mk_conj (t1, t2)
+  val term_exists =
+      prove(mk_exists(x, mk_comb(termP, x)),
+            EXISTS_TAC (list_mk_icomb(inst [beta |-> glam_ty] GVAR_t,
+                                      [mk_arb stringSyntax.string_ty,
+                                       mk_arb gvar_ty])) THEN
+            MATCH_MP_TAC (genind_rules |> SPEC_ALL |> CONJUNCT1) THEN
+            BETA_TAC THEN REWRITE_TAC [])
+  val term_bij_ax = new_type_definition (tyname, term_exists)
+  val newty = term_bij_ax |> concl |> dest_exists |> #1 |> type_of |> dom_rng |> #1
+  val term_ABSREP =
+      define_new_type_bijections { ABS = tyname ^ "_ABS", REP = tyname ^ "_REP",
+                                   name = tyname ^ "_ABSREP", tyax = term_bij_ax}
+  val absrep_id = term_ABSREP |> CONJUNCT1
+  val (term_ABS_t, term_REP_t) = let
+    val eqn1_lhs = absrep_id|> concl |> strip_forall |> #2 |> lhs
+    val (a, x) = dest_comb eqn1_lhs
+  in
+    (a, rator x)
+  end
+  fun term_ABSf x = mk_comb(term_ABS_t, x)
+  fun term_REPf x = mk_comb(term_REP_t, x)
+  val g = mk_var("g", newty) and h = mk_var("h", newty)
+  val term_ABS_pseudo11 = prove(
+    mk_imp(termPf x /\ termPf y, mk_eq(mk_eq(term_ABSf x, term_ABSf y), mk_eq(x,y))),
+    STRIP_TAC THEN EQ_TAC THENL [ALL_TAC, DISCH_THEN SUBST1_TAC THEN REFL_TAC] THEN
+    DISCH_THEN (MP_TAC o AP_TERM term_REP_t) THEN
+    REPEAT (POP_ASSUM (SUBST1_TAC o CONV_RULE (REWR_CONV (CONJUNCT2 term_ABSREP)))) THEN
+    REWRITE_TAC [])
+  val term_REP_11 = prove(
+    mk_eq(mk_eq(term_REPf g, term_REPf h), mk_eq(g,h)),
+    EQ_TAC THENL [ALL_TAC, DISCH_THEN SUBST1_TAC THEN REFL_TAC] THEN
+    DISCH_THEN (MP_TAC o AP_TERM term_ABS_t) THEN REWRITE_TAC [absrep_id])
+  val genind_term_REP = prove(
+    termPf (term_REPf g),
+    CONV_TAC (REWR_CONV (CONJUNCT2 term_ABSREP) THENC
+              LAND_CONV (RAND_CONV (REWR_CONV absrep_id))) THEN
+    REFL_TAC)
+  val genind_exists = prove(
+    mk_eq(termPf x, mk_exists(g, mk_eq(x, term_REPf g))),
+    EQ_TAC THENL [
+      REWRITE_TAC [CONJUNCT2 term_ABSREP] THEN DISCH_THEN (SUBST1_TAC o SYM) THEN
+      EXISTS_TAC (term_ABSf x) THEN REFL_TAC,
+      DISCH_THEN (X_CHOOSE_THEN g SUBST1_TAC) THEN
+      CONV_TAC (REWR_CONV (EQT_INTRO genind_term_REP))
+    ])
+  val repabs_pseudo_id =
+      term_ABSREP |> CONJUNCT2 |> SPEC_ALL |> EQ_IMP_RULE |> #1 |> GEN_ALL
+in
+  {term_ABS_pseudo11 = term_ABS_pseudo11,
+   term_REP_11 = term_REP_11, repabs_pseudo_id = repabs_pseudo_id,
+   absrep_id = absrep_id,
+   genind_term_REP = genind_term_REP,
+   genind_exists = genind_exists,
+   newty = newty,
+   termP = termP,
+   term_REP_t = term_REP_t, term_ABS_t = term_ABS_t}
+end
+
+
+fun termP_removal (info as {elimth,absrep_id,tpm_def,termP,repty}) t = let
+  val (v, body) = dest_forall t
+  fun ELIM_HERE t = let
+    val (v,body) = dest_forall t
+    val (h,c) = dest_imp body
+  in
+    BINDER_CONV (LAND_CONV
+                     (markerLib.move_conj_left (aconv (mk_comb(termP, v)))) THENC
+                     TRY_CONV (REWR_CONV (GSYM AND_IMP_INTRO)) THENC
+                     RAND_CONV (UNBETA_CONV v)) THENC
+    REWR_CONV elimth THENC BINDER_CONV BETA_CONV THENC
+    PURE_REWRITE_CONV [absrep_id, GSYM tpm_def]
+  end t
+
+in
+  if  Type.compare(type_of v, repty) = EQUAL then
+    (SWAP_FORALL_CONV THENC BINDER_CONV (termP_removal info)) ORELSEC
+    ELIM_HERE
+  else NO_CONV
+end t
+
+(* Vacuous FCBs are of the form
+     !vars.... . sideconds ==> v ∉ supp dpm (af args)
+   where none of the args are v, and where the sideconds are sufficient to establish
+   that v is not in the support of the args, nor in the support of af.
+
+   These arise from the encoding of non-binding recursive constructors with the GLAM
+   constructor, which introduces an unused binding name.
+*)
+
+fun impconcl t = t |> strip_forall |> #2 |> dest_imp |> #2
+val argcong = let
+  val fg = mk_eq(mk_var("f", alpha --> beta), mk_var("g", alpha --> beta))
+  val xy = mk_eq(mk_var("x", alpha), mk_var("y", alpha))
+  val (xy_th, fg_th) = CONJ_PAIR (ASSUME (mk_conj(xy, fg)))
+in
+  MK_COMB (fg_th, xy_th) |> DISCH_ALL |> GEN_ALL
+end
+
+val is_perm_t = prim_mk_const{Thy = "nomset", Name = "is_perm"}
+fun elim_vacuous_FCBs {finite_fv,tpm_is_perm} th = let
+  val h = hyp th
+  fun spot_vacuous t = let
+    val c = t |> impconcl |> dest_neg
+    val (v,supp_t) = pred_setSyntax.dest_in c
+  in
+    if free_in v supp_t then NONE else SOME(t,repeat rator (rand supp_t))
+  end handle HOL_ERR _ => NONE
+  val vacs = List.mapPartial spot_vacuous h
+  fun permfor v t = let
+    val c = t |> impconcl
+  in
+    Term.aconv v (repeat rator (rhs c))
+  end handle HOL_ERR _ => false
+  val vac_pms = map (fn (t,v) => (t,v,valOf (List.find (permfor v) h))) vacs
+  val finite_t = valOf (List.find pred_setSyntax.is_finite h)
+  val perm_t = valOf (List.find (same_const is_perm_t o rator) h)
+  fun GET_FRESH_SETS (asl,w) = let
+    val (_, bod) = dest_exists w
+    val vnotinA_c = last (strip_conj bod)
+    val v = lhand (dest_neg vnotinA_c)
+    fun getset t = let
+      val (v', s) = t |> dest_neg |> pred_setSyntax.dest_in
+    in
+      if aconv v' v then SOME s else NONE
+    end handle HOL_ERR _ => NONE
+    val sets = List.mapPartial getset asl
+  in
+    EXISTS_TAC (List.foldr pred_setSyntax.mk_union (hd sets) (tl sets))
+  end (asl,w)
+  open nomsetTheory
+  fun mk_result(goal,v,pm) =
+      TAC_PROOF(([], goal),
+                REPEAT GEN_TAC THEN STRIP_TAC THEN
+                MATCH_MP_TAC nomsetTheory.notinsupp_I THEN
+                GET_FRESH_SETS THEN REPEAT CONJ_TAC THENL [
+                  ACCEPT_TAC (ASSUME perm_t),
+                  REWRITE_TAC [ASSUME finite_t, finite_fv,
+                               pred_setTheory.FINITE_UNION],
+                  REWRITE_TAC [support_def, pred_setTheory.IN_UNION,
+                               DE_MORGAN_THM] THEN REPEAT STRIP_TAC THEN
+                  (fn (asl,w) =>
+                      MP_TAC (PART_MATCH (lhs o #2 o strip_imp) (ASSUME pm) (lhs w))
+                             (asl,w)) THEN
+                  ASM_REWRITE_TAC [] THEN DISCH_THEN SUBST1_TAC THEN
+                  REPEAT (MATCH_MP_TAC argcong THEN CONJ_TAC THEN1
+                            (MATCH_MP_TAC supp_fresh THEN
+                             ASM_REWRITE_TAC [tpm_is_perm, ASSUME perm_t] THEN
+                             CONJ_TAC THEN FIRST_X_ASSUM MATCH_MP_TAC THEN
+                             ASM_REWRITE_TAC [])) THEN
+                  REFL_TAC,
+                  ASM_REWRITE_TAC [pred_setTheory.IN_UNION]
+                ])
+  val elims = map mk_result vac_pms
+in
+  List.foldl (uncurry PROVE_HYP) th elims
+end
+
+fun lift_exfunction {repabs_pseudo_id, term_REP_t, cons_info} th = let
+  fun mk_conremove {con_termP, con_def} =
+      con_termP |> MATCH_MP repabs_pseudo_id
+                |> CONV_RULE (LAND_CONV (RAND_CONV (REWR_CONV (GSYM con_def))))
+                |> SYM
+  val conremoves = map mk_conremove cons_info
+  val f_REP_o = let
+    val (d,r) = dom_rng (type_of term_REP_t)
+    val f = mk_var("f", r --> Type.gen_tyvar())
+    val x = mk_var("x", d)
+  in
+    prove(
+      mk_eq(mk_comb(f, mk_comb(term_REP_t, x)),
+            mk_comb(combinSyntax.mk_o(f, term_REP_t), x)),
+      CONV_TAC (RAND_CONV (REWR_CONV combinTheory.o_THM)) THEN REFL_TAC)
+  end
+
+  fun fREPo_CONV t = let
+    val (v, bod) = dest_exists t
+    val o_t = combinSyntax.o_tm |> inst [alpha |-> Type.gen_tyvar()]
+    val fREPo = list_mk_icomb(o_t, [v, term_REP_t])
+  in
+    BINDER_CONV (UNBETA_CONV fREPo) t
+  end
+
+  fun elimfREPo th = let
+    val (v,bod) = dest_exists (concl th)
+    val (vnm, _) = dest_var v
+    val bod_th = ASSUME bod
+    val (P, arg) = dest_comb bod
+    val newf = mk_var(vnm, type_of arg)
+    val newbod = mk_comb(P, newf)
+  in
+    CHOOSE (v, th) (EXISTS (mk_exists(newf, newbod), arg) bod_th)
+           |> CONV_RULE (BINDER_CONV BETA_CONV)
+  end
+in
+  th |> REWRITE_RULE (f_REP_o::conremoves)
+     |> CONV_RULE fREPo_CONV
+     |> elimfREPo
+end
+
+fun sort_uvars t = let
+  val (v, bod) = dest_forall t
+  val (v', _) = dest_forall bod
+  val (nm1, ty1) = dest_var v
+  val (nm2, ty2) = dest_var v'
+  fun tycmp (ty1,ty2) =
+      if Type.compare(ty1,ty2) = EQUAL then EQUAL
+      else if Type.compare(ty1,``:string``) = EQUAL then LESS
+      else if is_vartype ty2 andalso not (is_vartype ty1) then LESS
+      else Type.compare(ty1, ty2)
+in
+  if pair_compare(tycmp,String.compare) ((ty1,nm1), (ty2,nm2)) = GREATER then
+    SWAP_FORALL_CONV
+  else NO_CONV
+end t
+
+fun rename_vars alist t = let
+  val (bv, _) = dest_abs t
+  val (v, _) = dest_var bv
+in
+  case Lib.total (Lib.assoc v) alist of
+    NONE => NO_CONV
+  | SOME v' => RENAME_VARS_CONV [v']
+end t
+
+fun prove_alpha_fcbhyp {ppm, alphas, rwts} th = let
+  open lcsymtacs nomsetTheory
+  val th = rpt_hyp_dest_conj (UNDISCH th)
+  fun foldthis (h,th) = let
+    val h_th =
+      TAC_PROOF(([], h),
+                rpt gen_tac >> strip_tac >>
+                FIRST (map (match_mp_tac o GSYM) alphas) >>
+                match_mp_tac (GEN_ALL notinsupp_fnapp) >>
+                EXISTS_TAC ppm >>
+                srw_tac [] rwts)
+  in
+    PROVE_HYP h_th th
+  end
+in
+  HOLset.foldl foldthis th (hypset th)
+end
+
+end (* struct *)
